phoas_lambda2.v
@@ -1,0 +1,145 @@
+From Stdlib Require Import Program.Equality.
+
+Definition name := nat.
+
+Inductive kind : Type :=
+  | kind_type : kind
+  | kind_lt : kind.
+
+Inductive type' {tvar : kind -> Type} : kind -> Type :=
+  | type_var' : forall {k}, tvar k -> type' k
+  | type_fun' : type' kind_type -> type' kind_type -> type' kind_type
+  | type_all' : forall {k}, (tvar k -> type' kind_type) -> type' kind_type.
+
+Hint Constructors type'.
+
+Definition type k := forall tvar, type' (tvar := tvar) k.
+Definition type1 (k_free : kind) (k_res : kind) := forall tvar, tvar k_free -> type' (tvar := tvar) k_res.
+Definition type_var {k} {tvar} (x : tvar k) := type_var' x.
+Definition type_fun (arg res : type kind_type) : type kind_type :=
+  fun tvar => type_fun' (arg tvar) (res tvar).
+Definition type_all {k : kind} (t : type1 k kind_type) : type kind_type :=
+  fun var => type_all' (fun x => t var x).
+
+Infix "-->" := type_fun' (right associativity, at level 60).
+Infix "c-->" := type_fun (right associativity, at level 60).
+
+Fixpoint flatten_type {tvar : kind -> Type} {k : kind} (t : type' k) {struct t} : type' k :=
+  match t with
+  | type_var' v => v
+  | type_fun' arg res => type_fun' (flatten_type arg) (flatten_type res)
+  | type_all' f => type_all' (fun x => flatten_type (f (type_var' (tvar := tvar) x)))
+  end.
+
+Definition subst_type' 
+  {k_arg} {k_res} {tvar : kind -> Type} 
+  (inner : type' (tvar := tvar) k_arg) (outer : type1 k_arg k_res) : type' k_res := 
+  flatten_type (outer type' inner).
+
+Example id_type_example : type kind_type := type_all (fun _ ty => type_var' ty --> type_var ty).
+
+Inductive term' 
+  {tvar : kind -> Type} {var : type' (tvar := tvar) kind_type -> Type} : 
+  type' (tvar := tvar) kind_type -> Type :=
+  | term_var' : forall {ty}, var ty -> term' ty
+  | term_app' : forall {arg} {res}, term' (arg --> res) -> term' arg -> term' res
+  | term_abs' : forall {arg} {res}, (var arg -> term' res) -> term' (arg --> res)
+  | term_tapp' :
+      forall {k_arg} {f : type1 k_arg kind_type} (t : term' (type_all' (f tvar))) (ty : type' k_arg), 
+      term' (subst_type' ty f)
+  | term_tabs' : forall {k_arg} {ty} (arg : tvar k_arg), term' (ty arg) -> term' (type_all' ty).
+
+Hint Constructors term'.
+Infix "@" := term_app' (left associativity, at level 50).
+Infix "t@" := term_tapp' (left associativity, at level 50).
+
+Example id_term_example : term' (type_all' (fun _ ty => type_var' ty --> type_var' ty)) :=
+  term_tabs' _ (fun x => term_abs' (fun y => term_var' y)).
+
+Definition term (ty : type' kind_type) := forall tvar var, term' (tvar := tvar) (var := var) ty.
+Definition term1 (ty_free : type kind_type) (ty : type kind_type) := 
+  forall var, var ty_free -> term' (var := var) ty. 
+Definition term_app {arg} {res} (f : term (arg --> res)) (arg : term arg) : term res :=
+  fun var => term_app' (f var) (arg var).
+Definition term_abs {arg} {res} (t : term1 arg res) : term (arg --> res) :=
+  fun var => term_abs' (fun x => t var x).
+Definition term_tapp 
+  {k_arg} {f : type1 k_arg kind_type}
+  (t : term (type_all f)) (ty : type k_arg) : term (subst_type ty f) :=
+  fun var => term_tapp' (t var) ty.
+Definition term_tabs
+  {k_arg} {f : type1 k_arg kind_type}
+  (t : term (type_all f)) : term (type_all f) :=
+  fun var => term_tabs' (t var).
+
+Fixpoint flatten 
+  {var : type kind_type -> Type} {ty : type kind_type} 
+  (t : term' (var := term') ty) {struct t} : term' ty :=
+  match t with
+  | term_var v => v
+  | term_app' f arg => term_app' (flatten f) (flatten arg)
+  | term_abs' f => term_abs' (fun x => flatten (f (term_var (var := var) x)))
+  | term_tapp' t ty => term_tapp' (flatten t) ty
+  | term_tabs' t => term_tabs' (flatten t)
+  end.
+
+Definition subst {ty1} {ty2} (inner : term ty1) (outer : term1 ty1 ty2) : term ty2 := 
+  fun var => flatten (outer (term' (var := var)) (inner var)).
+
+Inductive is_value : forall {ty}, term ty -> Prop :=
+  | is_value_abs : forall {arg} {res} (f : term1 arg res), is_value (term_abs f)
+  | is_value_tabs : forall {k_arg} {f : type1 k_arg kind_type} (t : term (type_all f)), is_value (term_tabs t).
+
+Hint Constructors is_value.
+
+Example id_example : term 
+  (type_all (k := kind_type) (fun _ ty => type_fun' (type_var ty) (type_var ty))) := 
+  term_tabs (fun _ ty => term_abs' (_)).
+
+Reserved Notation "t ==> t'" (no associativity, at level 90).
+Inductive step : forall {ty}, term ty -> term ty -> Prop :=
+  | step_beta :
+      forall arg res (f : term1 arg res) (v : term arg),
+      is_value v ->
+      term_app (term_abs f) v ==> subst v f
+  | step_app1 :
+      forall {arg} {res} {t1 : term (arg --> res)} {t1' : term (arg --> res)} {t2 : term arg},
+      t1 ==> t1' ->
+      step (ty := res) (term_app t1 t2) (term_app t1' t2)
+  | step_app2 :
+      forall {arg} {res} {t1 : term (arg --> res)} {t2 : term arg} {t2' : term arg},
+      t2 ==> t2' ->
+      step (ty := res) (term_app t1 t2) (term_app t1 t2')
+  where "t ==> t'" := (step t t').
+
+Hint Constructors step.
+
+Theorem preservation : forall {ty} (t t' : term ty),
+  step t t' ->
+  True.
+Proof. intros. trivial. Qed.
+
+Inductive closed_term : forall {ty}, term ty -> Prop :=
+  | closed_app : forall {arg} {res} (f : term (arg --> res)) (t : term arg),
+      closed_term f ->
+      closed_term t ->
+      closed_term (term_app f t)
+  | closed_abs : forall {arg} {res} (f : term1 arg res),
+      closed_term (term_abs f).
+
+Hint Constructors closed_term.
+
+Axiom every_term_closed : forall {ty} (t : term ty), closed_term t.
+
+Theorem progress : forall {ty} (t : term ty), 
+  closed_term t -> is_value t \/ (exists t', step t t').
+Proof. 
+  intros. 
+  induction H.
+  { destruct IHclosed_term1; auto; destruct IHclosed_term2; auto.
+    { right. inversion H1; subst. simpl_existT; subst. exists (subst t f0). eapply step_beta; auto. }
+    { right. destruct H2 as [t' Ht']. exists (term_app f t'). eapply step_app2; auto. }
+    { right. destruct H1 as [t' Ht']. exists (term_app t' t). eapply step_app1; auto. }
+    { right. destruct H1 as [f' Hf']. exists (term_app f' t). eapply step_app1; auto. } }
+  { left. constructor. }
+Qed.
